Implement set restriction

vale/specs/defs/Vale.Lib.Set.fst
@@ -2,6 +2,7 @@ module Vale.Lib.Set
 open FStar.Mul
 
 friend FStar.Map
+friend FStar.Set
 
 let rec remove_between' s (start:int) (finish:int{start <= finish}) : Tot (s':S.set int{ forall i.
   ((start <= i /\ i < finish) ==> not (S.mem i s')) /\
@@ -17,3 +18,9 @@ let remove_between s start finish =
 let remove_between_reveal s start finish i = ()
 
 let lemma_sel_restrict #a s m k = ()
+
+let set_restrict #t s p =
+  FStar.FunctionalExtensionality.on_dom t (fun x ->
+      s x && p x)
+
+let lemma_set_restrict #t s p = ()
